theories/coneris/examples/hash/con_hash_interface4.v
@@ -2,270 +2,86 @@ From clutch.coneris Require Import coneris.
 
 Set Default Proof Using "Type*".
 
-(*
-   A concurrent interface for hash functions with presampling
-   for individual keys
- *)
-
-
-Class con_hash4 `{!conerisGS Σ} (val_size max_key : nat ):= Con_Hash4
+(** A concurrent interface for hash functions with presampling for individual keys *)
+Class con_hash4 Σ `{!conerisGS Σ} := Con_Hash4
 {
   (** * Operations *)
   init_con_hash : val;
-  compute_con_hash : val;
-  (** * Ghost state *)
-
-  (** [name] is used to associate [locked] with [is_lock] *)
-  (* tape_name: Type; *)
 
   (** * Predicates *)
-  conhashfun (γs : gname * gname) (f : val) : iProp Σ;
-  hashkey (γs : gname * gname) (k : nat) (v : option nat) : iProp Σ;
+  conhashfun (γs : gname * gname * gname) (val_size : nat) (f : val) : iProp Σ;
+  hashkey (γs : gname * gname * gname) (k : nat) (v : option nat) : iProp Σ;
 
   (** * General properties of the predicates *)
-  (* #[global] concrete_seq_hash_timeless {L : seq_hashG Σ} f m :: *)
-  (*   Timeless (concrete_seq_hash (L:=L) f m); *)
-  #[global] hashkey_timeless γs k v ::
-    Timeless (hashkey γs k v);
-  #[global] conhashfun_persistent γs f ::
-    Persistent (conhashfun γs f);
-  #[global] hashkey_Some_persistent γs k v ::
-  Persistent (hashkey γs k (Some v));
-  hashkey_exclusive γs k v v' ::
-    hashkey γs k v -∗ hashkey γs k v'  -∗ False;
-  hash_key_valid γs k v n :
-    hashkey γs k v -∗ ⌜ v = Some n ⌝ -∗ ⌜ (n ≤ val_size)%nat ⌝;
+  #[global] hashkey_timeless γs k v :: Timeless (hashkey γs k v);
+  #[global] conhashfun_persistent γs vs f :: Persistent (conhashfun γs vs f);
+  #[global] hashkey_Some_persistent γs k v :: Persistent (hashkey γs k (Some v));
 
-  hashkey_presample E k (bad : gset nat) (ε εI εO: nonnegreal) γs :
-  (* Note: there should be no way for you to own a hashkey for
-     a key out of range, so this is redundant
-    k ≤ max_key →
-  *)
+  hashkey_presample k (bad : gset nat) (ε εI εO: nonnegreal) γs val_size f :
     (∀ x, x ∈ bad → x < S val_size) →
     (εI * size bad + εO * (val_size + 1 - size bad) <= ε * (val_size + 1))%R →
+    conhashfun γs val_size f -∗
     hashkey γs k None -∗
     ↯ ε -∗
-    state_update E E (∃ (n : fin (S val_size)),
-        ((⌜fin_to_nat n ∉ bad⌝ ∗ ↯ εO) ∨ (⌜fin_to_nat n ∈ bad⌝ ∗ ↯ εI)) ∗
-          hashkey γs k (Some (fin_to_nat n)));
+    state_update ⊤ ⊤ (∃ (n : fin (S val_size)),
+      ((⌜fin_to_nat n ∉ bad⌝ ∗ ↯ εO) ∨ (⌜fin_to_nat n ∈ bad⌝ ∗ ↯ εI)) ∗
+      hashkey γs k (Some (fin_to_nat n)));
 
-  conhash_init :
-  {{{ True }}}
-    init_con_hash #()
-  {{{ (γs : gname * gname) conhash, RET conhash;
-        conhashfun γs conhash ∗
-        ([∗ set] k ∈ (set_seq 0 (S max_key)), hashkey γs k None)  }}} ;
+  conhash_init val_size max :
+    {{{ True }}}
+      init_con_hash #val_size #max
+    {{{ γs conhash, RET conhash;
+        conhashfun γs val_size conhash ∗
+        ([∗ set] k ∈ (set_seq 0 (S max)), hashkey γs k None)  }}} ;
 
-  wp_conhashfun_prev f (k n : nat) γs :
-  {{{ conhashfun γs f ∗ hashkey γs k (Some n) }}}
-    f #k
-  {{{ RET #n; conhashfun γs f ∗ hashkey γs k (Some n) }}}
-
+  wp_conhashfun_prev f (k n : nat) γs val_size :
+    {{{ conhashfun γs val_size f ∗ hashkey γs k (Some n) }}}
+      f #k
+    {{{ RET #n; True }}}
 }.
 
-
 Section derived_lemmas.
-  Context `{conerisGS Σ, !con_hash4 val_size max_key}.
+  Context `{conerisGS Σ, !con_hash4 Σ}.
 
-Lemma wp_hash_lookup_safe k f γs :
-    {{{ hashkey γs k None ∗ conhashfun γs f }}}
-        f #k
-    {{{ (v : nat), RET #v; ⌜ (v ≤ val_size)%nat ⌝ ∗ hashkey γs k (Some v) ∗ conhashfun γs f }}}.
+  Lemma wp_hash_lookup_safe k f γs val_size :
+    {{{ hashkey γs k None ∗ conhashfun γs val_size f }}}
+      f #k
+    {{{ (v : nat), RET #v; ⌜(v ≤ val_size)%nat⌝ ∗ hashkey γs k (Some v) }}}.
   Proof.
     iIntros (Φ) "(HNone & #Hinv) HΦ".
     iMod (ec_zero) as "Herr".
     iApply state_update_pgl_wp.
-    iMod (hashkey_presample _ _ ∅ nnreal_zero nnreal_zero nnreal_zero with "HNone [Herr]")
-        as "(%v & _ & Hhauth)"; auto.
-      + set_solver.
-      + rewrite size_empty /=.
-        lra.
-      + iModIntro.
-        wp_apply (wp_conhashfun_prev with "[-HΦ]"); auto.
-        iIntros "(?&?)".
-        iApply "HΦ".
-        iFrame.
-        iPureIntro.
-        pose proof (fin_to_nat_lt v).
-        lia.
-   Qed.
+    iMod (hashkey_presample _ ∅ nnreal_zero nnreal_zero nnreal_zero with "Hinv HNone [Herr]")
+      as "(%v & _ & #Hkey)"; auto.
+    - set_solver.
+    - rewrite size_empty /=. lra.
+    - iModIntro.
+      wp_apply (wp_conhashfun_prev with "[-HΦ]"); auto.
+      iIntros "_". iApply "HΦ". iFrame "#". iPureIntro.
+      pose proof (fin_to_nat_lt v). lia.
+  Qed.
 
-
-Lemma wp_hash_lookup_avoid_set k f γs (bad : gset nat)(ε εI εO:nonnegreal) :
-    (forall x : nat, x ∈ bad -> (x < S val_size)%nat) ->
-    (εI * (size bad) + εO * (val_size + 1 - size bad) <= ε * (val_size + 1))%R ->
-    {{{ ↯ ε ∗ hashkey γs k None ∗ conhashfun γs f }}}
+  Lemma wp_hash_lookup_avoid_set k f γs (bad : gset nat)(ε εI εO:nonnegreal) val_size :
+    (∀ x : nat, x ∈ bad → (x < S val_size)%nat) →
+    (εI * (size bad) + εO * (val_size + 1 - size bad) <= ε * (val_size + 1))%R →
+    {{{ ↯ ε ∗ hashkey γs k None ∗ conhashfun γs val_size f }}}
       f #k
-      {{{ (v : nat), RET #v; ⌜ (v ≤ val_size)%nat ⌝ ∗
-                             ((⌜v ∈ bad⌝) ∗ ↯ εI  ∨
-                                (⌜v ∉ bad⌝) ∗ ↯ εO) ∗
-                             hashkey γs k (Some v) }}}.
+    {{{ (v : nat), RET #v;
+        ⌜(v ≤ val_size)%nat⌝ ∗
+        ((⌜v ∈ bad⌝) ∗ ↯ εI  ∨ (⌜v ∉ bad⌝) ∗ ↯ εO) ∗
+        hashkey γs k (Some v) }}}.
   Proof.
     iIntros (Hbad Hdistr Φ) "(Herr & Hnone & #Hinv) HΦ".
     iApply state_update_pgl_wp.
-    iMod (hashkey_presample _ _ bad ε εI εO with "Hnone [Herr]")
-      as "(%v & Hv & Hhauth)"; auto.
+    iMod (hashkey_presample _ bad ε εI εO with "Hinv Hnone [Herr]")
+      as "(%v & Hv & #Hhauth)"; auto.
     iModIntro.
-    wp_apply (wp_conhashfun_prev with "[-HΦ Hv]"); auto.
-    iIntros "(?&?)".
-    iApply "HΦ".
-    iFrame.
-    iSplit.
-    {
-      iPureIntro.
-      pose proof (fin_to_nat_lt v).
-      lia.
-    }
+    wp_apply (wp_conhashfun_prev with "[$]").
+    iIntros "Hf".
+    iApply "HΦ". iFrame.
+    iSplit; [iPureIntro|].
+    { pose proof (fin_to_nat_lt v). lia. }
     iDestruct "Hv" as "[?|?]"; auto.
   Qed.
 
 End derived_lemmas.
-
-(*
-
-Old interface
-
-Class con_hash4 `{!conerisGS Σ} (val_size max_key : nat ):= Con_Hash4
-{
-  (** * Operations *)
-  init_hash4 : val;
-  compute_hash4 : val;
-  (** * Ghost state *)
-
-  (** [name] is used to associate [locked] with [is_lock] *)
-  (* tape_name: Type; *)
-
-  hash_view_gname:Type;
-  hash_lock_gname:Type;
-
-  (** * Predicates *)
-  con_hash_inv4 (N:namespace) (f l hm: val) (R:gmap nat nat -> iProp Σ) {HR: ∀ m, Timeless (R m )} (γ1:hash_view_gname) (γ_lock:hash_lock_gname): iProp Σ;
-  hash_auth4 (m:gmap nat nat) (γ:hash_view_gname) : iProp Σ;
-  hash_frag4 (k v : nat) (γ:hash_view_gname) : iProp Σ;
-
-  (** * General properties of the predicates *)
-  (* #[global] concrete_seq_hash_timeless {L : seq_hashG Σ} f m :: *)
-  (*   Timeless (concrete_seq_hash (L:=L) f m); *)
-  #[global] hash_auth_timeless m γ ::
-    Timeless (hash_auth4 m γ );
-  #[global] hash_frag_timeless v res γ ::
-    Timeless (hash_frag4 v res γ );
-  #[global] con_hash_inv_persistent N f l hm γ1 R {HR: ∀ m, Timeless (R m )}  γ_lock ::
-    Persistent (con_hash_inv4 N f l hm R γ1 γ_lock);
-  #[global] hash_frag_persistent k v γ ::
-    Persistent (hash_frag4 k v γ );
-  hash_auth_exclusive m m' γ :
-    hash_auth4 m γ  -∗ hash_auth4 m' γ  -∗ False;
-  hash_auth_frag_agree m k v γ :
-    hash_auth4 m γ  -∗ hash_frag4 k v γ  -∗ ⌜m!!k=Some v⌝;
-  hash_auth_duplicate m k v γ :
-    m!!k=Some v -> hash_auth4 m γ  -∗ hash_frag4 k v γ ;
-  hash_frag_frag_agree k v1 v2 γ :
-    hash_frag4 k v1 γ  -∗ hash_frag4 k v2 γ  -∗ ⌜v1=v2⌝;
-  hash_frag_valid k v γ :
-    hash_frag4 k v γ -∗ ⌜ (v ≤ val_size)%nat ⌝;
-
-
-  hash_preview4 N k f l hm R {HR: ∀ m, Timeless (R m )}  m γ_hv γ_lock (bad : gset nat)(ε εI εO:nonnegreal) E:
-  ↑(N) ⊆ E ->
-  (forall x : nat, x ∈ bad -> (x < S val_size)%nat) ->
-  (εI * (size bad) + εO * (val_size + 1 - size bad) <= ε * (val_size + 1))%R ->
-  hash_auth4 m γ_hv -∗
-  con_hash_inv4 N f l hm R γ_hv γ_lock -∗
-  ⌜ m !! k = None ⌝ -∗
-  ↯ ε -∗
-    state_update E E (∃ (n:fin(S val_size)),
-          ( (⌜fin_to_nat n ∈ bad⌝) ∗ ↯ εI  ∨
-            (⌜fin_to_nat n ∉ bad⌝) ∗ ↯ εO
-          )∗
-          hash_auth4 (<[k:=fin_to_nat n]> m) γ_hv);
-
-
-  con_hash_init4 N R {HR: ∀ m, Timeless (R m)} :
-    {{{ R ∅ }}}
-      init_hash4 #()
-      {{{ (f:val), RET f; ∃ l hm γ1 γ_lock, con_hash_inv4 N f l hm R γ1 γ_lock ∗
-                                                  hash_auth4 ∅ γ1
-      }}} ;
-
-
-  con_hash_spec4 N f l hm R {HR: ∀ m, Timeless (R m)} γ1 γ_lock (k:nat) v:
-  {{{ con_hash_inv4 N f l hm R γ1 γ_lock ∗
-       hash_frag4 k v γ1
-  }}}
-      f #k
-      {{{ (res:nat), RET (#res);  ⌜ res = v ⌝
-      }}}
-
-}.
-
-
-Section derived_lemmas.
-  Context `{conerisGS Σ, !con_hash4 val_size max_key}.
-
-  Lemma wp_hash_lookup_safe N k f l hm m R {HR: ∀ m, Timeless (R m )} γhv γlock :
-    (k ≤ max_key)%nat ->
-    {{{ hash_auth4 m γhv ∗ con_hash_inv4 N f l hm R γhv γlock }}}
-        f #k
-    {{{ (v : nat), RET #v; ⌜ (v ≤ val_size)%nat ⌝ ∗ hash_auth4 (<[k:=v]> m) γhv }}}.
-  Proof.
-    iIntros (Hk Φ) "(Hhauth & #Hinv) HΦ".
-    destruct (m !! k) as [v|] eqn:Hlookup.
-    - iPoseProof (hash_auth_duplicate m k v with "Hhauth") as "#Hfrag"; auto.
-      wp_apply con_hash_spec4; auto.
-      iPoseProof (hash_frag_valid with "Hfrag") as "%".
-      iIntros (?) "->".
-      iApply "HΦ".
-      iSplit; auto.
-      by rewrite insert_id.
-    - iMod (ec_zero) as "Herr".
-      iApply state_update_pgl_wp.
-      iMod (hash_preview4 N _  _ _ _ _ _ _ _ ∅ nnreal_zero nnreal_zero nnreal_zero with "Hhauth [] [] [Herr]")
-        as "(%v & _ & Hhauth)"; auto.
-      + set_solver.
-      + rewrite size_empty /=.
-        lra.
-      + iModIntro.
-        iPoseProof (hash_auth_duplicate _ k v with "Hhauth") as "#Hfrag"; auto.
-        {
-          rewrite lookup_insert //.
-        }
-        wp_apply con_hash_spec4; auto.
-        iPoseProof (hash_frag_valid with "Hfrag") as "%".
-        iIntros (?) "->".
-        iApply "HΦ".
-        iSplit; auto.
-   Qed.
-
-  Lemma wp_hash_lookup_avoid_set N k f l hm m R {HR: ∀ m, Timeless (R m )} γhv γlock (bad : gset nat)(ε εI εO:nonnegreal) :
-    (forall x : nat, x ∈ bad -> (x < S val_size)%nat) ->
-    (εI * (size bad) + εO * (val_size + 1 - size bad) <= ε * (val_size + 1))%R ->
-    (k ≤ max_key)%nat ->
-    m !! k = None ->
-    {{{ ↯ ε ∗ hash_auth4 m γhv ∗ con_hash_inv4 N f l hm R γhv γlock }}}
-      f #k
-      {{{ (v : nat), RET #v; ⌜ (v ≤ val_size)%nat ⌝ ∗
-                             ((⌜v ∈ bad⌝) ∗ ↯ εI  ∨
-                                (⌜v ∉ bad⌝) ∗ ↯ εO) ∗
-                             hash_auth4 (<[k:=v]> m) γhv }}}.
-  Proof.
-    iIntros (Hbad Hdistr Hk Hnone Φ) "(Herr & Hhauth & #Hinv) HΦ".
-    iApply state_update_pgl_wp.
-    iMod (hash_preview4 N _  _ _ _ _ _ _ _ bad ε εI εO with "Hhauth [] [] [Herr]")
-      as "(%v & Hv & Hhauth)"; auto.
-    iModIntro.
-    iPoseProof (hash_auth_duplicate _ k v with "Hhauth") as "#Hfrag"; auto.
-    {
-      rewrite lookup_insert //.
-    }
-    wp_apply con_hash_spec4; auto.
-    iPoseProof (hash_frag_valid with "Hfrag") as "%".
-    iIntros (?) "->".
-    iApply "HΦ".
-    iSplit; auto.
-    by iFrame.
-  Qed.
-
-End derived_lemmas.
-
-*)
